erasure/theories/EInversion.v
@@ -23,7 +23,7 @@ Local Existing Instance default_checker_flags.
 Lemma type_Case_inv (Σ : global_env_ext) (hΣ : wf Σ.1) Γ ind npar p c brs T :
   Σ;;; Γ |- PCUICAst.tCase (ind, npar) p c brs : T ->
   { '(u, args, mdecl, idecl, pty, indctx, pctx, ps, btys) : _ &
-         (PCUICTyping.declared_inductive (fst Σ) mdecl ind idecl) *
+         (PCUICReduction.declared_inductive (fst Σ) mdecl ind idecl) *
          (PCUICAst.ind_npars mdecl = npar) *
          let pars := firstn npar args in
          (Σ;;; Γ |- p : pty) *
@@ -37,13 +37,13 @@ Proof.
   intros. dependent induction X.
   - unshelve eexists.
     + repeat refine (_,_). all:shelve.
-    + cbn. subst pars. intuition eauto.
+    + cbn. subst pars. intuition eauto. reflexivity.
   - edestruct (IHX hΣ _ _ _ _ _ eq_refl) as [ [[[[[[[[]]]]]]]] ].
     repeat match goal with [ H : _ * _ |- _ ] => destruct H end.
     unshelve eexists.
     + repeat refine (_, _). all:shelve.
     + cbn. intuition eauto.
-      all: eapply PCUICConversion.cumul_trans; eauto.
+      all: eapply PCUICConfluence.cumul_trans; eauto.
 Qed.
 
 Notation type_Construct_inv := PCUICInversion.inversion_Construct.
