erasure/theories/ErasureFunction.v
@@ -349,7 +349,7 @@ Next Obligation.
 
      eapply conv_context_refl; eauto. econstructor.
 
-     eapply PCUICConversion.conv_sym, red_conv; eauto.
+     eapply conv_sym, red_conv; eauto.
 
   ++ sq. etransitivity. eassumption.
 
@@ -359,7 +359,7 @@ Next Obligation.
 
      econstructor.
 
-     eapply PCUICConversion.conv_sym, red_conv; eauto.
+     eapply conv_sym, red_conv; eauto.
 Qed.
 Next Obligation.
   Hint Constructors squash. destruct HΣ.
@@ -419,8 +419,6 @@ Next Obligation.
        eapply type_reduction in X0; eauto.
 
        eapply principal_typing in c0 as (? & ? & ? & ?). 2:eauto. 2:{ exact X0. }
-
-       eapply cumul_prop1 in c; eauto.
 
        destruct (invert_cumul_sort_r _ _ _ _ c0) as (? & ? & ?).
        destruct (invert_cumul_sort_r _ _ _ _ c1) as (? & ? & ?).
