pcuic/theories/PCUICConversionLemmas.v
@@ -1,0 +1,888 @@
+(* Distributed under the terms of the MIT license.   *)
+From Equations Require Import Equations.
+From Coq Require Import Bool String List Program BinPos Compare_dec Omega Lia.
+From MetaCoq.Template Require Import config utils AstUtils.
+From MetaCoq.PCUIC Require Import PCUICAst PCUICAstUtils PCUICInduction
+     PCUICLiftSubst PCUICUnivSubst PCUICEquality
+     PCUICTyping PCUICWeakeningEnv PCUICWeakening PCUICSubstitution
+     PCUICCumulativity PCUICConfluence PCUICParallelReductionConfluence
+     PCUICEquality PCUICContextConversion.
+
+Require Import ssreflect ssrbool.
+Require Import String.
+From MetaCoq Require Import LibHypsNaming.
+Local Open Scope string_scope.
+Set Asymmetric Patterns.
+Require Import CRelationClasses.
+Require Import Equations.Type.Relation Equations.Type.Relation_Properties.
+Require Import Equations.Prop.DepElim.
+
+Ltac tc := try typeclasses eauto 10.
+(* Hint Resolve eq_universe_leq_universe' : pcuic. *)
+
+
+Derive Signature for cumul.
+
+Lemma congr_cumul_prod : forall `{checker_flags} Σ Γ na na' M1 M2 N1 N2,
+    Σ ;;; Γ |- M1 = N1 ->
+    Σ ;;; (Γ ,, vass na M1) |- M2 <= N2 ->
+    Σ ;;; Γ |- (tProd na M1 M2) <= (tProd na' N1 N2).
+Proof.
+  intros.
+Admitted.
+
+(* Should follow from context conversion + invariants on T and U *)
+(* Lemma conv_conv_alt `{cf : checker_flags} {Σ : global_env_ext} (wfΣ : wf Σ) Γ T U : *)
+(*   Σ ;;; Γ |- T = U -> Σ ;;; Γ |- T == U. *)
+(* Proof. *)
+(* Admitted. *)
+
+Lemma cumul_Sort_inv {cf:checker_flags} Σ Γ s s' :
+  Σ ;;; Γ |- tSort s <= tSort s' -> leq_universe (global_ext_constraints Σ) s s'.
+Proof.
+  intros H; depind H; auto.
+  - now inversion l.
+  - depelim r. solve_discr.
+  - depelim r. solve_discr.
+Qed.
+
+Lemma cumul_Sort_Prod_inv {cf:checker_flags} Σ Γ s na dom codom :
+  Σ ;;; Γ |- tSort s <= tProd na dom codom -> False.
+Proof.
+  intros H; depind H; auto.
+  - now inversion l.
+  - depelim r. solve_discr.
+  - depelim r. solve_discr. eapply IHcumul. reflexivity.
+    eapply IHcumul. reflexivity.
+Qed.
+
+Lemma cumul_Sort_l_inv {cf:checker_flags} Σ Γ s T :
+  Σ ;;; Γ |- tSort s <= T ->
+  ∑ s', red Σ Γ T (tSort s') * leq_universe Σ s s'.
+Proof.
+  intros H; depind H; auto.
+  - now inversion l.
+  - depelim r. solve_discr.
+  - destruct IHcumul as [s' [redv leq]].
+    exists s'. split; auto. now eapply red_step with v.
+Qed.
+
+Lemma cumul_Sort_r_inv {cf:checker_flags} Σ Γ s T :
+  Σ ;;; Γ |- T <= tSort s ->
+  ∑ s', red Σ Γ T (tSort s') * leq_universe Σ s' s.
+Proof.
+  intros H; depind H; auto.
+  - now inversion l.
+  - destruct IHcumul as [s' [redv leq]].
+    exists s'. split; auto. now eapply red_step with v.
+  - depelim r. solve_discr.
+Qed.
+
+Lemma cumul_LetIn_l_inv {cf:checker_flags} (Σ : global_env_ext) Γ na b B codom T :
+  wf Σ ->
+  Σ ;;; Γ |- tLetIn na b B codom <= T ->
+  ∑ codom', red Σ Γ T codom' *
+                     (Σ ;;; Γ |- codom {0 := b} <= codom').
+Proof.
+  intros wfΣ H; depind H; auto.
+  - inv l. eexists (u' {0 := t'}); intuition eauto. eapply red1_red. constructor.
+    transitivity (codom {0 := t'}).
+    { constructor. eapply eq_term_upto_univ_subst; trivial. auto with pcuic. reflexivity. }
+    constructor. now eapply subst_leq_term.
+  - depelim r.
+    * exists u; intuition auto.
+    * solve_discr.
+    * specialize (IHcumul _ _ _ _ _ wfΣ eq_refl).
+      destruct IHcumul as [codom' [reddom' leq]].
+      exists codom'; intuition auto.
+      transitivity (codom {0 := r}); eauto.
+      eapply red_cumul. eapply (red_red Σ _ [vdef na b B] []) => //. constructor. now eapply red1_red.
+      constructor. rewrite -{1}(subst_empty 0 b). repeat constructor.
+    * specialize (IHcumul _ _ _ _ _ wfΣ eq_refl).
+      destruct IHcumul as [codom' [reddom' leq]].
+      exists codom'; intuition auto.
+    * specialize (IHcumul _ _ _ _ _ wfΣ eq_refl).
+      destruct IHcumul as [codom' [reddom' leq]].
+      exists codom'; intuition auto.
+      eapply transitivity; [|eassumption].
+      eapply red_cumul.
+      rewrite -{1 2}(subst_empty 0 b).
+      eapply (untyped_substitution_red _ _ [vdef na b B] []); auto. repeat constructor.
+  - specialize (IHcumul wfΣ).
+    destruct IHcumul as [codom' [reddom' leq]] => //.
+    exists codom'; intuition auto.
+    now eapply red_step with v.
+Qed.
+
+Lemma cumul_LetIn_r_inv {cf:checker_flags} (Σ : global_env_ext) Γ na b B codom T :
+  wf Σ ->
+  Σ ;;; Γ |- T <= tLetIn na b B codom ->
+  ∑ codom', red Σ Γ T codom' *
+                     (Σ ;;; Γ |- codom' <= codom {0 := b}).
+Proof.
+  intros wfΣ H; depind H; auto.
+  - inv l. eexists (u {0 := t0}); intuition eauto. eapply red1_red. constructor.
+    transitivity (codom {0 := t0}).
+    { constructor. eapply eq_term_upto_univ_subst; trivial. auto with pcuic. reflexivity. }
+    constructor. eapply eq_term_upto_univ_subst; auto with pcuic. reflexivity.
+  - specialize (IHcumul wfΣ).
+    destruct IHcumul as [codom' [reddom' leq]] => //.
+    exists codom'; intuition auto.
+    now eapply red_step with v.
+  - depelim r.
+    * eexists ; intuition eauto.
+    * solve_discr.
+    * specialize (IHcumul _ _ _ _ _ wfΣ eq_refl).
+      destruct IHcumul as [codom' [reddom' leq]].
+      exists codom'; intuition auto.
+      transitivity (codom {0 := r}); eauto.
+      eapply red_cumul_inv. eapply (red_red Σ _ [vdef na b B] []) => //. constructor. now eapply red1_red.
+      constructor. rewrite -{1}(subst_empty 0 b). repeat constructor.
+    * specialize (IHcumul _ _ _ _ _ wfΣ eq_refl).
+      destruct IHcumul as [codom' [reddom' leq]].
+      exists codom'; intuition auto.
+    * specialize (IHcumul _ _ _ _ _ wfΣ eq_refl).
+      destruct IHcumul as [codom' [reddom' leq]].
+      exists codom'; intuition auto.
+      eapply transitivity; [eassumption|].
+      eapply red_cumul_inv.
+      rewrite -{1 2}(subst_empty 0 b).
+      eapply (untyped_substitution_red _ _ [vdef na b B] []); auto. repeat constructor.
+Qed.
+
+Lemma cumul_Prod_l_inv {cf:checker_flags} (Σ : global_env_ext) Γ na dom codom T :
+  wf Σ ->
+  Σ ;;; Γ |- tProd na dom codom <= T ->
+  ∑ na' dom' codom', red Σ Γ T (tProd na' dom' codom') *
+                     (Σ ;;; Γ |- dom = dom') * (Σ ;;; Γ ,, vass na dom |- codom <= codom').
+Proof.
+  intros wfΣ H; depind H; auto.
+  - inv l. exists na', a', b'; intuition eauto; constructor; auto.
+  - depelim r. solve_discr.
+    * specialize (IHcumul _ _ _ _ wfΣ eq_refl).
+      destruct IHcumul as [na' [dom' [codom' [[reddom' eqdom'] leq]]]].
+      exists na', dom', codom'; intuition auto.
+      transitivity N1; eauto. now econstructor 2.
+      eapply cumul_conv_ctx; eauto. constructor. reflexivity.
+      constructor. symmetry; eapply red_conv; auto.
+
+    * specialize (IHcumul _ _ _ _ wfΣ eq_refl).
+      destruct IHcumul as [na' [dom' [codom' [[reddom' eqdom'] leq]]]].
+      exists na', dom', codom'; intuition auto.
+      transitivity N2; eauto. eapply red_cumul; auto.
+  - destruct IHcumul as [na' [dom' [codom' [[reddom' eqdom'] leq]]]] => //.
+    exists na', dom', codom'; intuition auto.
+    now eapply red_step with v.
+Qed.
+
+Lemma cumul_Prod_r_inv {cf:checker_flags} (Σ : global_env_ext) Γ na' dom' codom' T :
+  wf Σ ->
+  Σ ;;; Γ |- T <= tProd na' dom' codom' ->
+  ∑ na dom codom, red Σ Γ T (tProd na dom codom) *
+                     (Σ ;;; Γ |- dom = dom') * (Σ ;;; Γ ,, vass na' dom' |- codom <= codom').
+Proof.
+  intros wfΣ H; depind H; auto.
+  - inv l. exists na, a, b; intuition eauto; constructor; auto.
+  - destruct IHcumul as [na [dom [codom [[reddom' eqdom'] leq]]]] => //.
+    exists na, dom, codom; intuition auto.
+    now eapply red_step with v.
+  - depelim r. solve_discr.
+    * specialize (IHcumul _ _ _ _ wfΣ eq_refl).
+      destruct IHcumul as [na [dom [codom [[reddom' eqdom'] leq]]]].
+      eexists _, _, _; intuition eauto.
+      transitivity N1; eauto. symmetry; apply red_conv; auto.
+      eapply cumul_conv_ctx; eauto. constructor. reflexivity.
+      constructor. symmetry. eapply red_conv; auto.
+
+    * specialize (IHcumul _ _ _ _ wfΣ eq_refl).
+      destruct IHcumul as [na [dom [codom [[reddom' eqdom'] leq]]]].
+      eexists _, _, _; intuition eauto.
+      transitivity N2; eauto. eapply red_cumul_inv; auto.
+Qed.
+
+Lemma cumul_Prod_Sort_inv {cf:checker_flags} Σ Γ s na dom codom :
+  Σ ;;; Γ |- tProd na dom codom <= tSort s -> False.
+Proof.
+  intros H; depind H; auto.
+  - now inversion l.
+  - depelim r. solve_discr. eapply IHcumul; reflexivity.
+    eapply IHcumul; reflexivity.
+  - depelim r. solve_discr.
+Qed.
+
+Lemma cumul_Prod_Prod_inv {cf:checker_flags} (Σ : global_env_ext) Γ na na' dom dom' codom codom' : wf Σ ->
+  Σ ;;; Γ |- tProd na dom codom <= tProd na' dom' codom' ->
+   ((Σ ;;; Γ |- dom = dom') * (Σ ;;; Γ ,, vass na' dom' |- codom <= codom'))%type.
+Proof.
+  intros wfΣ H; depind H; auto.
+  - inv l. split; auto; constructor; auto.
+  - depelim r. solve_discr.
+    destruct (IHcumul na na' N1 _ _ _ wfΣ eq_refl).
+    split; auto. transitivity N1=> //. now eapply red_conv, red1_red.
+    destruct (IHcumul na na' _ _ N2 _ wfΣ eq_refl).
+    split; auto. eapply cumul_trans. auto. 2:eauto.
+    eapply cumul_conv_ctx; eauto. eapply red_cumul; eauto.
+    constructor. reflexivity. auto with pcuic.
+  - depelim r. solve_discr.
+    destruct (IHcumul na na' _ _ _ _ wfΣ eq_refl).
+    split; auto. transitivity N1 => //. symmetry => //.
+    now eapply red_conv, red1_red.
+    eapply cumul_red_ctx_inv. auto. eauto. constructor. eapply All2_local_env_red_refl. red.
+    now eapply red1_red.
+    destruct (IHcumul na na' _ _ _ _ wfΣ eq_refl).
+    split; auto.
+    eapply cumul_trans with N2; auto.
+    (* eapply red1_red, red_conv in r. apply conv_cumul_inv. , r. *)
+(* Qed. *)
+Admitted.
+
+Lemma assumption_context_app Γ Γ' :
+  assumption_context (Γ' ,,, Γ) ->
+  assumption_context Γ * assumption_context Γ'.
+Proof.
+  induction Γ; simpl; split; try constructor; auto. depelim H. constructor; auto. now eapply IHΓ.
+  depelim H. now eapply IHΓ.
+Qed.
+
+Lemma it_mkProd_or_LetIn_ass_inv {cf : checker_flags} (Σ : global_env_ext) Γ ctx ctx' s s' :
+  wf Σ ->
+  assumption_context ctx ->
+  assumption_context ctx' ->
+  Σ ;;; Γ |- it_mkProd_or_LetIn ctx (tSort s) <= it_mkProd_or_LetIn ctx' (tSort s') ->
+  conv_context Σ ctx ctx' * leq_term Σ (tSort s) (tSort s').
+Proof.
+  intros wfΣ.
+  revert Γ ctx' s s'.
+  induction ctx using rev_ind.
+  intros. destruct ctx' using rev_ind. simpl in X.
+  - eapply cumul_Sort_inv in X. split; constructor; auto.
+  - destruct x as [na [b|] ty]. elimtype False.
+    apply assumption_context_app in H0.
+    destruct H0. inv a0.
+    rewrite it_mkProd_or_LetIn_app in X.
+    apply assumption_context_app in H0 as [H0 _].
+    specialize (IHctx' H0).
+    simpl in IHctx'. simpl in X. unfold mkProd_or_LetIn in X. simpl in X.
+    eapply cumul_Sort_Prod_inv in X. depelim X.
+  - intros.
+    rewrite it_mkProd_or_LetIn_app in X.
+    simpl in X.
+    eapply assumption_context_app in H as [H H'].
+    destruct x as [na [b|] ty]. elimtype False. inv H'.
+    rewrite /mkProd_or_LetIn /= in X.
+    destruct ctx' using rev_ind.
+    simpl in X.
+    now eapply cumul_Prod_Sort_inv in X.
+    eapply assumption_context_app in H0 as [H0 Hx].
+    destruct x as [na' [b'|] ty']; [elimtype False; inv Hx|].
+    rewrite it_mkProd_or_LetIn_app in X.
+    rewrite /= /mkProd_or_LetIn /= in X.
+    eapply cumul_Prod_Prod_inv in X as [Hdom Hcodom]; auto.
+    specialize (IHctx (Γ ,, vass na' ty') l0 s s' H H0 Hcodom). clear IHctx'.
+    intuition auto.
+Admitted.
+
+(** Injectivity of products, the essential property of cumulativity needed for subject reduction. *)
+Lemma cumul_Prod_inv {cf:checker_flags} Σ Γ na na' A B A' B' :
+  wf Σ.1 -> wf_local Σ Γ ->
+  Σ ;;; Γ |- tProd na A B <= tProd na' A' B' ->
+   ((Σ ;;; Γ |- A = A') * (Σ ;;; Γ ,, vass na' A' |- B <= B'))%type.
+Proof.
+  intros wfΣ wfΓ H; depind H.
+  - depelim l.
+    split; auto.
+    now constructor.
+    now constructor.
+
+  - depelim r. solve_discr.
+    specialize (IHcumul _ _ _ _ _ _ wfΣ wfΓ eq_refl).
+    intuition auto.
+    econstructor 2; eauto.
+
+    specialize (IHcumul _ _ _ _ _ _ wfΣ wfΓ eq_refl).
+    intuition auto. apply cumul_trans with N2. auto.
+    eapply cumul_conv_ctx; eauto.
+
+    econstructor 2. eauto. constructor. reflexivity.
+    constructor. now apply conv_ctx_refl.
+    constructor; auto.
+    auto.
+
+  - depelim r. solve_discr.
+    specialize (IHcumul _ _ _ _ _ _ wfΣ wfΓ eq_refl).
+    intuition auto. econstructor 3. 2:eauto. auto.
+    eapply cumul_conv_ctx in b. eauto. auto. constructor. eapply conv_ctx_refl. auto.
+    constructor. econstructor 3; tea. reflexivity.
+
+    specialize (IHcumul _ _ _ _ _ _ wfΣ wfΓ eq_refl).
+    intuition auto. apply cumul_trans with N2. auto. auto.
+    eapply cumul_red_r; eauto. reflexivity.
+Qed.
+
+Lemma tProd_it_mkProd_or_LetIn na A B ctx s :
+  tProd na A B = it_mkProd_or_LetIn ctx (tSort s) ->
+  { ctx' & ctx = (ctx' ++ [vass na A])%list /\
+           destArity [] B = Some (ctx', s) }.
+Proof.
+  intros. exists (removelast ctx).
+  revert na A B s H.
+  induction ctx using rev_ind; intros; noconf H.
+  rewrite it_mkProd_or_LetIn_app in H. simpl in H.
+  destruct x as [na' [b'|] ty']; noconf H; simpl in *.
+  rewrite removelast_app. congruence. simpl. rewrite app_nil_r. intuition auto.
+  rewrite destArity_it_mkProd_or_LetIn. simpl. now rewrite app_context_nil_l.
+Qed.
+
+Section Inversions.
+  Context {cf : checker_flags}.
+  Context (Σ : global_env_ext) (wfΣ : wf Σ).
+
+  Lemma cumul_App_r {Γ f u v} :
+    Σ ;;; Γ |- u = v ->
+    Σ ;;; Γ |- tApp f u <= tApp f v.
+  Proof.
+    intros h.
+    induction h.
+    - eapply cumul_refl. constructor.
+      + apply leq_term_refl.
+      + assumption.
+    -  eapply cumul_red_l ; try eassumption.
+       econstructor. assumption.
+    - eapply cumul_red_r ; try eassumption.
+      econstructor. assumption.
+  Qed.
+
+  Lemma conv_App_r {Γ f x y} :
+    Σ ;;; Γ |- x = y ->
+    Σ ;;; Γ |- tApp f x = tApp f y.
+  Proof.
+    intros h.
+    induction h.
+    - constructor. constructor.
+      + apply eq_term_refl.
+      + assumption.
+    - eapply conv_red_l ; eauto.
+      econstructor. assumption.
+    - eapply conv_red_r ; eauto.
+      econstructor. assumption.
+  Qed.
+
+  Lemma conv_Prod_l:
+    forall {Γ na na' A1 A2 B},
+      Σ ;;; Γ |- A1 = A2 ->
+      Σ ;;; Γ |- tProd na A1 B = tProd na' A2 B.
+  Proof.
+    intros Γ na na' A1 A2 B h.
+    induction h.
+    - constructor. constructor.
+      + assumption.
+      + apply eq_term_refl.
+    - eapply conv_red_l ; eauto.
+      econstructor. assumption.
+    - eapply conv_red_r ; eauto.
+      econstructor. assumption.
+  Qed.
+
+  Lemma conv_Prod_r  :
+    forall {Γ na A B1 B2},
+      Σ ;;; Γ ,, vass na A |- B1 = B2 ->
+      Σ ;;; Γ |- tProd na A B1 = tProd na A B2.
+  Proof.
+    intros Γ na A B1 B2 h.
+    induction h.
+    - constructor. constructor.
+      + apply eq_term_refl.
+      + assumption.
+    - eapply conv_red_l ; eauto.
+      econstructor. assumption.
+    - eapply conv_red_r ; eauto.
+      econstructor. assumption.
+  Qed.
+
+  Lemma cumul_Prod_r :
+    forall {Γ na A B1 B2},
+      Σ ;;; Γ ,, vass na A |- B1 <= B2 ->
+      Σ ;;; Γ |- tProd na A B1 <= tProd na A B2.
+  Proof.
+    intros Γ na A B1 B2 h.
+    induction h.
+    - eapply cumul_refl. constructor.
+      + apply eq_term_refl.
+      + assumption.
+    - eapply cumul_red_l ; try eassumption.
+      econstructor. assumption.
+    - eapply cumul_red_r ; try eassumption.
+      econstructor. assumption.
+  Qed.
+
+  Global Instance conv_cum_refl :
+    forall leq Γ, RelationClasses.Reflexive (conv_cum leq Σ Γ).
+  Proof.
+    intros leq Γ t.
+    destruct leq; now constructor.
+  Qed.
+
+  Global Instance conv_cum_trans :
+    forall leq Γ, RelationClasses.Transitive (conv_cum leq Σ Γ).
+  Proof.
+    intros leq Γ u v w h1 h2.
+    destruct leq.
+    - cbn in *. destruct h1, h2. constructor.
+      eapply conv_trans ; eassumption.
+    - cbn in *. destruct h1, h2. constructor. eapply cumul_trans ; eassumption.
+  Qed.
+
+  Lemma red_conv_cum_l :
+    forall leq Γ u v,
+      red (fst Σ) Γ u v ->
+      conv_cum leq Σ Γ u v.
+  Proof.
+    intros leq Γ u v h.
+    induction h.
+    - reflexivity.
+    - etransitivity; tea.
+      destruct leq.
+      + simpl. destruct IHh. constructor.
+        eapply conv_red_l; eauto. reflexivity.
+      + simpl. constructor.
+        now eapply cumul_red_l.
+  Qed.
+
+  Lemma red_conv_cum_r :
+    forall leq Γ u v,
+      red (fst Σ) Γ u v ->
+      conv_cum leq Σ Γ v u.
+  Proof.
+    intros leq Γ u v h.
+    induction h.
+    - reflexivity.
+    - etransitivity; tea.
+      destruct leq.
+      + simpl. destruct IHh. constructor.
+        eapply conv_red_r; eauto. reflexivity.
+      + simpl. constructor.
+        now eapply cumul_red_r.
+  Qed.
+
+  Lemma conv_cum_Prod leq Γ na1 na2 A1 A2 B1 B2 :
+      Σ ;;; Γ |- A1 = A2 ->
+      conv_cum leq Σ (Γ,, vass na1 A1) B1 B2 ->
+      conv_cum leq Σ Γ (tProd na1 A1 B1) (tProd na2 A2 B2).
+  Proof.
+    intros h1 h2; destruct leq.
+    - simpl in *. destruct h2 as [h2]. constructor.
+      eapply conv_trans => //.
+      + eapply conv_Prod_r. eassumption.
+      + eapply conv_Prod_l. eassumption.
+    - simpl in *. destruct h2 as [h2]. constructor.
+      eapply cumul_trans. auto.
+      + eapply cumul_Prod_r. eassumption.
+      + eapply conv_cumul. eapply conv_Prod_l. assumption.
+  Qed.
+
+  Lemma cumul_Case_c :
+    forall Γ indn p brs u v,
+      Σ ;;; Γ |- u = v ->
+      Σ ;;; Γ |- tCase indn p u brs <= tCase indn p v brs.
+  Proof.
+    intros Γ [ind n] p brs u v h.
+    induction h.
+    - constructor. constructor.
+      + eapply eq_term_refl.
+      + assumption.
+      + eapply All2_same.
+        intros. split ; eauto.
+        reflexivity.
+    - eapply cumul_red_l ; eauto.
+      constructor. assumption.
+    - eapply cumul_red_r ; eauto.
+      constructor. assumption.
+  Qed.
+
+  Lemma cumul_Proj_c :
+    forall Γ p u v,
+      Σ ;;; Γ |- u = v ->
+      Σ ;;; Γ |- tProj p u <= tProj p v.
+  Proof.
+    intros Γ p u v h.
+    induction h.
+    - eapply cumul_refl. constructor. assumption.
+    - eapply cumul_red_l ; try eassumption.
+      econstructor. assumption.
+    - eapply cumul_red_r ; try eassumption.
+      econstructor. assumption.
+  Qed.
+
+  Lemma conv_App_l :
+    forall {Γ f g x},
+      Σ ;;; Γ |- f = g ->
+      Σ ;;; Γ |- tApp f x = tApp g x.
+  Proof.
+    intros Γ f g x h.
+    induction h.
+    - constructor. constructor.
+      + assumption.
+      + apply eq_term_refl.
+    - eapply conv_red_l ; eauto.
+      econstructor. assumption.
+    - eapply conv_red_r ; eauto.
+      econstructor. assumption.
+  Qed.
+
+  Lemma App_conv :
+    forall Γ t1 t2 u1 u2,
+      Σ ;;; Γ |- t1 = t2 ->
+      Σ ;;; Γ |- u1 = u2 ->
+      Σ ;;; Γ |- tApp t1 u1 = tApp t2 u2.
+  Proof.
+    intros. etransitivity.
+    eapply conv_App_l; tea.
+    eapply conv_App_r; tea.
+  Qed.
+
+  Lemma conv_Case_c :
+    forall Γ indn p brs u v,
+      Σ ;;; Γ |- u = v ->
+      Σ ;;; Γ |- tCase indn p u brs = tCase indn p v brs.
+  Proof.
+    intros Γ [ind n] p brs u v h.
+    induction h.
+    - constructor. constructor.
+      + eapply eq_term_refl.
+      + assumption.
+      + eapply All2_same.
+        intros. split ; eauto. reflexivity.
+    - eapply conv_red_l ; eauto.
+      constructor. assumption.
+    - eapply conv_red_r ; eauto.
+      constructor. assumption.
+  Qed.
+
+  Lemma conv_Proj_c :
+    forall Γ p u v,
+      Σ ;;; Γ |- u = v ->
+      Σ ;;; Γ |- tProj p u = tProj p v.
+  Proof.
+    intros Γ p u v h.
+    induction h.
+    - eapply conv_refl. constructor. assumption.
+    - eapply conv_red_l ; try eassumption.
+      econstructor. assumption.
+    - eapply conv_red_r ; try eassumption.
+      econstructor. assumption.
+  Qed.
+
+  Lemma conv_Lambda_l :
+    forall Γ na A b na' A',
+      Σ ;;; Γ |- A = A' ->
+      Σ ;;; Γ |- tLambda na A b = tLambda na' A' b.
+  Proof.
+    intros Γ na A b na' A' h.
+    induction h.
+    - eapply conv_refl. constructor.
+      + assumption.
+      + eapply eq_term_refl.
+    - eapply conv_red_l ; try eassumption.
+      econstructor. assumption.
+    - eapply conv_red_r ; try eassumption.
+      econstructor. assumption.
+  Qed.
+
+  Lemma conv_Lambda_r :
+    forall Γ na A b b',
+      Σ ;;; Γ,, vass na A |- b = b' ->
+      Σ ;;; Γ |- tLambda na A b = tLambda na A b'.
+  Proof.
+    intros Γ na A b b' h.
+    induction h.
+    - eapply conv_refl. constructor.
+      + eapply eq_term_refl.
+      + assumption.
+    - eapply conv_red_l ; try eassumption.
+      econstructor. assumption.
+    - eapply conv_red_r ; try eassumption.
+      econstructor. assumption.
+  Qed.
+
+  Lemma cumul_LetIn_bo :
+    forall Γ na ty t u u',
+      Σ ;;; Γ ,, vdef na ty t |- u <= u' ->
+      Σ ;;; Γ |- tLetIn na ty t u <= tLetIn na ty t u'.
+  Proof.
+    intros Γ na ty t u u' h.
+    induction h.
+    - eapply cumul_refl. constructor.
+      all: try eapply eq_term_refl.
+      assumption.
+    - eapply cumul_red_l ; try eassumption.
+      econstructor. assumption.
+    - eapply cumul_red_r ; try eassumption.
+      econstructor. assumption.
+  Qed.
+
+  Lemma cumul_Lambda_r :
+    forall Γ na A b b',
+      Σ ;;; Γ,, vass na A |- b <= b' ->
+      Σ ;;; Γ |- tLambda na A b <= tLambda na A b'.
+  Proof.
+    intros Γ na A b b' h.
+    induction h.
+    - eapply cumul_refl. constructor.
+      + eapply eq_term_refl.
+      + assumption.
+    - eapply cumul_red_l ; try eassumption.
+      econstructor. assumption.
+    - eapply cumul_red_r ; try eassumption.
+      econstructor. assumption.
+  Qed.
+
+  Lemma cumul_it_mkLambda_or_LetIn :
+    forall Δ Γ u v,
+      Σ ;;; (Δ ,,, Γ) |- u <= v ->
+      Σ ;;; Δ |- it_mkLambda_or_LetIn Γ u <= it_mkLambda_or_LetIn Γ v.
+  Proof.
+    intros Δ Γ u v h. revert Δ u v h.
+    induction Γ as [| [na [b|] A] Γ ih ] ; intros Δ u v h.
+    - assumption.
+    - simpl. cbn. eapply ih.
+      eapply cumul_LetIn_bo. assumption.
+    - simpl. cbn. eapply ih.
+      eapply cumul_Lambda_r. assumption.
+  Qed.
+
+  Lemma cumul_it_mkProd_or_LetIn :
+    forall Δ Γ B B',
+      Σ ;;; (Δ ,,, Γ) |- B <= B' ->
+      Σ ;;; Δ |- it_mkProd_or_LetIn Γ B <= it_mkProd_or_LetIn Γ B'.
+  Proof.
+    intros Δ Γ B B' h.
+    induction Γ as [| [na [b|] A] Γ ih ] in Δ, B, B', h |- *.
+    - assumption.
+    - simpl. cbn. eapply ih.
+      eapply cumul_LetIn_bo. assumption.
+    - simpl. cbn. eapply ih.
+      eapply cumul_Prod_r. assumption.
+  Qed.
+
+  Lemma mkApps_conv_weak :
+    forall Γ u1 u2 l,
+      Σ ;;; Γ |- u1 = u2 ->
+      Σ ;;; Γ |- mkApps u1 l = mkApps u2 l.
+  Proof.
+    intros Γ u1 u2 l. induction l in u1, u2 |- *; cbn. trivial.
+    intros X. apply IHl. now apply conv_App_l.
+  Qed.
+
+
+  Lemma context_relation_length P Γ Γ' :
+    context_relation P Γ Γ' -> #|Γ| = #|Γ'|.
+  Proof.
+    induction 1; cbn; congruence.
+  Qed.
+
+
+  Lemma conv_cum_Lambda leq Γ na1 na2 A1 A2 t1 t2 :
+      Σ ;;; Γ |- A1 = A2 ->
+      conv_cum leq Σ (Γ ,, vass na1 A1) t1 t2 ->
+      conv_cum leq Σ Γ (tLambda na1 A1 t1) (tLambda na2 A2 t2).
+  Proof.
+    intros X H. destruct leq; cbn in *; sq.
+    - etransitivity. eapply conv_Lambda_r; tea.
+      now eapply conv_Lambda_l.
+    - etransitivity. eapply cumul_Lambda_r; tea.
+      eapply conv_cumul, conv_Lambda_l; tea.
+  Qed.
+
+  Lemma conv_LetIn_tm Γ na na' ty t t' u :
+      Σ ;;; Γ |- t = t' ->
+      Σ ;;; Γ |- tLetIn na t ty u = tLetIn na' t' ty u.
+  Proof.
+    induction 1.
+    - constructor 1. constructor; try reflexivity.
+      assumption.
+    - econstructor 2; tea. now constructor.
+    - econstructor 3; tea. now constructor.
+  Qed.
+
+  Lemma conv_LetIn_ty Γ na na' ty ty' t u :
+      Σ ;;; Γ |- ty = ty' ->
+      Σ ;;; Γ |- tLetIn na t ty u = tLetIn na' t ty' u.
+  Proof.
+    induction 1.
+    - constructor 1. constructor; try reflexivity.
+      assumption.
+    - econstructor 2; tea. now constructor.
+    - econstructor 3; tea. now constructor.
+  Qed.
+
+  Lemma conv_LetIn_bo Γ na ty t u u' :
+      Σ ;;; Γ ,, vdef na ty t |- u = u' ->
+      Σ ;;; Γ |- tLetIn na ty t u = tLetIn na ty t u'.
+  Proof.
+    induction 1.
+    - constructor 1. now constructor. 
+    - econstructor 2; tea. now constructor.
+    - econstructor 3; tea. now constructor.
+  Qed.
+
+  Lemma conv_cum_LetIn leq Γ na1 na2 t1 t2 A1 A2 u1 u2 :
+      Σ;;; Γ |- t1 = t2 ->
+      Σ;;; Γ |- A1 = A2 ->
+      conv_cum leq Σ (Γ ,, vdef na1 t1 A1) u1 u2 ->
+      conv_cum leq Σ Γ (tLetIn na1 t1 A1 u1) (tLetIn na2 t2 A2 u2).
+  Proof.
+    intros X H H'. destruct leq; cbn in *; sq.
+    - etransitivity. eapply conv_LetIn_bo; tea.
+      etransitivity. eapply conv_LetIn_tm; tea.
+      eapply conv_LetIn_ty with (na := na1); tea.
+    - etransitivity. eapply cumul_LetIn_bo; tea.
+      etransitivity. eapply conv_cumul, conv_LetIn_tm; tea.
+      eapply conv_cumul, conv_LetIn_ty with (na := na1); tea.
+  Qed.
+
+  Lemma conv_cum_conv_ctx leq Γ Γ' T U :
+    conv_cum leq Σ Γ T U ->
+    conv_context Σ Γ Γ' ->
+    conv_cum leq Σ Γ' T U.
+  Proof.
+    destruct leq; cbn; intros; sq.
+    eapply conv_conv_ctx; eassumption.
+    eapply cumul_conv_ctx; eassumption.
+  Qed.
+
+
+  Lemma it_mkLambda_or_LetIn_conv_cum leq Γ Δ1 Δ2 t1 t2 :
+      conv_context Σ (Γ ,,, Δ1) (Γ ,,, Δ2) ->
+      conv_cum leq Σ (Γ ,,, Δ1) t1 t2 ->
+      conv_cum leq Σ Γ (it_mkLambda_or_LetIn Δ1 t1) (it_mkLambda_or_LetIn Δ2 t2).
+  Proof.
+    induction Δ1 in Δ2, t1, t2 |- *; intros X Y.
+    - apply context_relation_length in X.
+      destruct Δ2; cbn in *; [trivial|].
+      rewrite app_length in X; lia.
+    - apply context_relation_length in X as X'.
+      destruct Δ2 as [|c Δ2]; simpl in *; [rewrite app_length in X'; lia|].
+      dependent destruction X.
+      + eapply IHΔ1; tas; cbn.
+        inv c0. eapply conv_cum_Lambda; tea.
+      + eapply IHΔ1; tas; cbn.
+        inversion c0; subst; eapply conv_cum_LetIn; auto. reflexivity.
+  Qed.
+
+  Lemma conv_it_mkProd_or_LetIn :
+    forall Δ Γ B B',
+      Σ ;;; (Δ ,,, Γ) |- B = B' ->
+      Σ ;;; Δ |- it_mkProd_or_LetIn Γ B = it_mkProd_or_LetIn Γ B'.
+  Proof.
+    intros Δ Γ B B' h.
+    induction Γ as [| [na [b|] A] Γ ih ] in Δ, B, B', h |- *.
+    - assumption.
+    - simpl. cbn. eapply ih.
+      eapply conv_LetIn_bo. assumption.
+    - simpl. cbn. eapply ih.
+      eapply conv_Prod_r. assumption.
+  Qed.
+
+  Lemma it_mkLambda_or_LetIn_conv Γ Δ1 Δ2 t1 t2 :
+      conv_context Σ (Γ ,,, Δ1) (Γ ,,, Δ2) ->
+      Σ ;;; Γ ,,, Δ1 |- t1 = t2 ->
+      Σ ;;; Γ |- it_mkLambda_or_LetIn Δ1 t1 = it_mkLambda_or_LetIn Δ2 t2.
+  Proof.
+    induction Δ1 in Δ2, t1, t2 |- *; intros X Y.
+    - apply context_relation_length in X.
+      destruct Δ2; cbn in *; [trivial|].
+      exfalso. rewrite app_length in X; lia.
+    - apply context_relation_length in X as X'.
+      destruct Δ2 as [|c Δ2]; simpl in *; [exfalso; rewrite app_length in X'; lia|].
+      dependent destruction X.
+      + eapply IHΔ1; tas; cbn.
+        inv c0. etransitivity. eapply conv_Lambda_r; tea.
+        now eapply conv_Lambda_l.
+      + eapply IHΔ1; tas; cbn.
+        etransitivity. eapply conv_LetIn_bo; tea. inv c0.
+        eapply conv_LetIn_ty; tea.
+        etransitivity. eapply conv_LetIn_tm; tea.
+        eapply conv_LetIn_ty with (na := na); tea.
+  Qed.
+
+  Lemma conv_it_mkLambda_or_LetIn :
+    forall Δ Γ B B',
+      Σ ;;; (Δ ,,, Γ) |- B = B' ->
+      Σ ;;; Δ |- it_mkLambda_or_LetIn Γ B = it_mkLambda_or_LetIn Γ B'.
+  Proof.
+    intros Δ Γ B B' h.
+    induction Γ as [| [na [b|] A] Γ ih ] in Δ, B, B', h |- *.
+    - assumption.
+    - simpl. cbn. eapply ih.
+      eapply conv_LetIn_bo. assumption.
+    - simpl. cbn. eapply ih.
+      eapply conv_Lambda_r. assumption.
+  Qed.
+
+  Lemma red_lambda_inv Γ na A1 b1 T :
+    red Σ Γ (tLambda na A1 b1) T ->
+    ∑ A2 b2, (T = tLambda na A2 b2) *
+             red Σ Γ A1 A2 * red Σ (Γ ,, vass na A1) b1 b2.
+  Proof.
+    intros.
+    eapply red_alt in X. eapply clos_rt_rt1n_iff in X.
+    depind X.
+    - eexists _, _; intuition eauto.
+    - depelim r; solve_discr; specialize (IHX _ _ _ _ eq_refl);
+      destruct IHX as [A2 [B2 [[-> ?] ?]]].
+      * eexists _, _; intuition eauto.
+        now eapply red_step with M'.
+        eapply PCUICConfluence.red_red_ctx; eauto.
+        constructor; auto. eapply All2_local_env_red_refl.
+        red. auto.
+      * eexists _, _; intuition eauto.
+        now eapply red_step with M'.
+  Qed.
+
+  Lemma Lambda_conv_cum_inv :
+    forall leq Γ na1 na2 A1 A2 b1 b2,
+      wf_local Σ Γ ->
+      conv_cum leq Σ Γ (tLambda na1 A1 b1) (tLambda na2 A2 b2) ->
+      ∥ Σ ;;; Γ |- A1 = A2 ∥ /\ conv_cum leq Σ (Γ ,, vass na1 A1) b1 b2.
+  Proof.
+    intros * wfΓ.
+    destruct leq; simpl in *.
+    - destruct 1.
+      eapply conv_alt in X as [l [r [redl [redr eq]]]].
+      eapply red_lambda_inv in redl as [A1' [b1' [[-> ?] ?]]].
+      eapply red_lambda_inv in redr as [A2' [b2' [[-> ?] ?]]].
+      depelim eq. assert (Σ ;;; Γ |- A1 = A2).
+      { eapply conv_trans with A1'; auto.
+        now apply red_conv.
+        eapply conv_trans with A2'; auto.
+        constructor. assumption.
+        symmetry; now apply red_conv. }
+      split; constructor; auto.
+      eapply conv_trans with b1'; auto.
+      now apply red_conv.
+      eapply conv_trans with b2'; auto.
+      constructor; auto.
+      apply conv_sym; auto.
+      eapply conv_conv_ctx; eauto.
+      now apply red_conv.
+      constructor; auto. reflexivity. constructor. now apply conv_sym.
+    - destruct 1.
+      eapply cumul_alt in X as [l [r [redl [redr eq]]]].
+      eapply red_lambda_inv in redl as [A1' [b1' [[-> ?] ?]]].
+      eapply red_lambda_inv in redr as [A2' [b2' [[-> ?] ?]]].
+      depelim eq. assert (Σ ;;; Γ |- A1 = A2).
+      { eapply conv_trans with A1'; auto.
+        now apply red_conv.
+        eapply conv_trans with A2'; auto.
+        constructor. assumption.
+        symmetry; now apply red_conv. }
+      split; constructor; auto.
+      eapply red_cumul_cumul; tea.
+      eapply cumul_trans with b2'; auto.
+      constructor; auto.
+      eapply cumul_conv_ctx; tas. eapply red_cumul_cumul_inv; tea.
+      reflexivity. symmetry in X.
+      constructor. reflexivity. now constructor.
+  Qed.
+
+End Inversions.
