pcuic/theories/PCUICSafeLemmata.v
@@ -10,7 +10,7 @@ From MetaCoq.PCUIC Require Import PCUICAst PCUICAstUtils PCUICInduction
      PCUICAlpha PCUICNormal PCUICInversion PCUICCumulativity PCUICReduction
      PCUICConfluence PCUICConversion PCUICContextConversion PCUICValidity
      PCUICParallelReductionConfluence PCUICWeakeningEnv
-     PCUICClosed PCUICPrincipality PCUICSubstitution
+     PCUICClosed PCUICPrincipality PCUICSubstitution PCUICConversionLemmas
      PCUICWeakening PCUICGeneration PCUICUtils.
 
 From Equations Require Import Equations.
@@ -515,91 +515,22 @@ Section Lemmata.
       Σ ;;; Γ |- zippx u ρ <= zippx v ρ.
   Proof.
     intros Γ u v ρ h.
-    revert u v h. induction ρ ; intros u v h.
-    - cbn. assumption.
-    - unfold zippx. simpl.
-      case_eq (decompose_stack ρ). intros l π e.
+    revert u v h. induction ρ ; intros u v h; unfold zippx; simpl.
+    all: eauto using cumul_it_mkLambda_or_LetIn.
+    - case_eq (decompose_stack ρ). intros l π e.
       unfold zippx in IHρ. rewrite e in IHρ.
       apply IHρ.
       eapply cumul_App_l. assumption.
-    - unfold zippx. simpl.
-      eapply cumul_it_mkLambda_or_LetIn.
-      assumption.
-    - unfold zippx. simpl.
-      eapply cumul_it_mkLambda_or_LetIn.
-      assumption.
-    - unfold zippx. simpl.
-      eapply cumul_it_mkLambda_or_LetIn.
-      assumption.
-    - unfold zippx. simpl.
-      eapply cumul_it_mkLambda_or_LetIn.
-      assumption.
-    - unfold zippx. simpl.
-      eapply cumul_it_mkLambda_or_LetIn.
-      assumption.
-    - unfold zippx. simpl.
-      eapply cumul_it_mkLambda_or_LetIn. cbn.
-      eapply cumul_Lambda_r.
-      assumption.
-    - unfold zippx. simpl.
-      eapply cumul_it_mkLambda_or_LetIn.
-      assumption.
-    - unfold zippx. simpl.
-      eapply cumul_it_mkLambda_or_LetIn. cbn.
-      eapply cumul_Lambda_r.
-      assumption.
-    - unfold zippx. simpl.
-      eapply cumul_it_mkLambda_or_LetIn. assumption.
-  Qed.
-
-  Lemma conv_LetIn_bo :
-    forall Γ na ty t u u',
-      Σ ;;; Γ ,, vdef na ty t |- u == u' ->
-      Σ ;;; Γ |- tLetIn na ty t u == tLetIn na ty t u'.
-  Proof.
-    intros Γ na ty t u u' h.
-    induction h.
-    - eapply conv_alt_refl. constructor.
-      all: try eapply eq_term_refl.
-      assumption.
-    - eapply conv_alt_red_l ; try eassumption.
-      econstructor. assumption.
-    - eapply conv_alt_red_r ; try eassumption.
-      econstructor. assumption.
-  Qed.
-
-  Lemma conv_alt_it_mkLambda_or_LetIn :
-    forall Δ Γ u v,
-      Σ ;;; (Δ ,,, Γ) |- u == v ->
-      Σ ;;; Δ |- it_mkLambda_or_LetIn Γ u == it_mkLambda_or_LetIn Γ v.
-  Proof.
-    intros Δ Γ u v h. revert Δ u v h.
-    induction Γ as [| [na [b|] A] Γ ih ] ; intros Δ u v h.
-    - assumption.
-    - simpl. cbn. eapply ih.
-      eapply conv_LetIn_bo. assumption.
-    - simpl. cbn. eapply ih.
-      eapply conv_Lambda_r. assumption.
-  Qed.
-
-  Lemma conv_alt_it_mkProd_or_LetIn :
-    forall Δ Γ B B',
-      Σ ;;; (Δ ,,, Γ) |- B == B' ->
-      Σ ;;; Δ |- it_mkProd_or_LetIn Γ B == it_mkProd_or_LetIn Γ B'.
-  Proof.
-    intros Δ Γ B B' h.
-    induction Γ as [| [na [b|] A] Γ ih ] in Δ, B, B', h |- *.
-    - assumption.
-    - simpl. cbn. eapply ih.
-      eapply conv_LetIn_bo. assumption.
-    - simpl. cbn. eapply ih.
-      eapply conv_Prod_r. assumption.
+    - eapply cumul_it_mkLambda_or_LetIn. cbn.
+      now eapply cumul_Lambda_r.
+    - eapply cumul_it_mkLambda_or_LetIn. cbn.
+      now eapply cumul_Lambda_r.
   Qed.
 
   Lemma conv_zipp :
     forall Γ u v ρ,
-      Σ ;;; Γ |- u == v ->
-      Σ ;;; Γ |- zipp u ρ == zipp v ρ.
+      Σ ;;; Γ |- u = v ->
+      Σ ;;; Γ |- zipp u ρ = zipp v ρ.
   Proof.
     intros Γ u v ρ h.
     unfold zipp.
@@ -622,10 +553,10 @@ Section Lemmata.
     - simpl.  eapply IHl. eapply cumul_App_l. assumption.
   Qed.
 
-  Lemma conv_zipp' :
+  Lemma conv_cum_zipp' :
     forall leq Γ u v π,
-      conv leq Σ Γ u v ->
-      conv leq Σ Γ (zipp u π) (zipp v π).
+      conv_cum leq Σ Γ u v ->
+      conv_cum leq Σ Γ (zipp u π) (zipp v π).
   Proof.
     intros leq Γ u v π h.
     destruct leq.
@@ -635,59 +566,34 @@ Section Lemmata.
 
   Lemma conv_alt_zippx :
     forall Γ u v ρ,
-      Σ ;;; (Γ ,,, stack_context ρ) |- u == v ->
-      Σ ;;; Γ |- zippx u ρ == zippx v ρ.
+      Σ ;;; (Γ ,,, stack_context ρ) |- u = v ->
+      Σ ;;; Γ |- zippx u ρ = zippx v ρ.
   Proof.
     intros Γ u v ρ h.
-    revert u v h. induction ρ ; intros u v h.
-    - cbn. assumption.
-    - unfold zippx. simpl.
-      case_eq (decompose_stack ρ). intros l π e.
+    revert u v h. induction ρ ; intros u v h; unfold zippx; simpl.
+    all: eauto using conv_it_mkLambda_or_LetIn.
+    - case_eq (decompose_stack ρ). intros l π e.
       unfold zippx in IHρ. rewrite e in IHρ.
       apply IHρ.
       eapply conv_App_l. assumption.
-    - unfold zippx. simpl.
-      eapply conv_alt_it_mkLambda_or_LetIn.
-      assumption.
-    - unfold zippx. simpl.
-      eapply conv_alt_it_mkLambda_or_LetIn.
-      assumption.
-    - unfold zippx. simpl.
-      eapply conv_alt_it_mkLambda_or_LetIn.
-      assumption.
-    - unfold zippx. simpl.
-      eapply conv_alt_it_mkLambda_or_LetIn.
-      assumption.
-    - unfold zippx. simpl.
-      eapply conv_alt_it_mkLambda_or_LetIn.
-      assumption.
-    - unfold zippx. simpl.
-      eapply conv_alt_it_mkLambda_or_LetIn. cbn.
-      eapply conv_Lambda_r.
-      assumption.
-    - unfold zippx. simpl.
-      eapply conv_alt_it_mkLambda_or_LetIn.
-      assumption.
-    - unfold zippx. simpl.
-      eapply conv_alt_it_mkLambda_or_LetIn. cbn.
-      eapply conv_Lambda_r.
-      assumption.
-    - unfold zippx. simpl.
-      eapply conv_alt_it_mkLambda_or_LetIn. assumption.
+    - eapply conv_it_mkLambda_or_LetIn. cbn.
+      now eapply conv_Lambda_r.
+    - eapply conv_it_mkLambda_or_LetIn. cbn.
+      now eapply conv_Lambda_r.
   Qed.
 
   Lemma conv_zippx :
     forall Γ u v ρ,
-      Σ ;;; Γ ,,, stack_context ρ |- u == v ->
-      Σ ;;; Γ |- zippx u ρ == zippx v ρ.
+      Σ ;;; Γ ,,, stack_context ρ |- u = v ->
+      Σ ;;; Γ |- zippx u ρ = zippx v ρ.
   Proof.
     intros Γ u v ρ uv. eapply conv_alt_zippx ; assumption.
   Qed.
 
-  Lemma conv_zippx' :
+  Lemma conv_cum_zippx' :
     forall Γ leq u v ρ,
-      conv leq Σ (Γ ,,, stack_context ρ) u v ->
-      conv leq Σ Γ (zippx u ρ) (zippx v ρ).
+      conv_cum leq Σ (Γ ,,, stack_context ρ) u v ->
+      conv_cum leq Σ Γ (zippx u ρ) (zippx v ρ).
   Proof.
     intros Γ leq u v ρ h.
     destruct leq.
@@ -1156,8 +1062,6 @@ Section Lemmata.
     assumption.
   Qed.
 
-  Hint Resolve conv_alt_refl conv_alt_red : core.
-  Hint Resolve conv_ctx_refl: core.
 
 
   (* Let bindings are not injective, so it_mkLambda_or_LetIn is not either.
@@ -1242,7 +1146,7 @@ Section Lemmata.
     forall Γ u v A B,
       Σ ;;; Γ |- u : A ->
       Σ ;;; Γ |- v : B ->
-      Σ ;;; Γ |- u == v ->
+      Σ ;;; Γ |- u = v ->
       ∑ C,
         Σ ;;; Γ |- u : C ×
         Σ ;;; Γ |- v : C.
@@ -1263,7 +1167,7 @@ Section Lemmata.
     forall Γ u v π,
       welltyped Σ Γ (zipc v π) ->
       welltyped Σ (Γ ,,, stack_context π) u ->
-      Σ ;;; Γ ,,, stack_context π |- u == v ->
+      Σ ;;; Γ ,,, stack_context π |- u = v ->
       welltyped Σ Γ (zipc u π).
   Proof.
     destruct hΣ as [wΣ].
@@ -1288,7 +1192,7 @@ Section Lemmata.
     forall Γ u v π,
       wellformed Σ Γ (zipc v π) ->
       wellformed Σ (Γ ,,, stack_context π) u ->
-      Σ ;;; Γ ,,, stack_context π |- u == v ->
+      Σ ;;; Γ ,,, stack_context π |- u = v ->
       wellformed Σ Γ (zipc u π).
   Admitted.
 
@@ -1394,17 +1298,17 @@ Section Lemmata.
     assumption.
   Qed.
 
-  Lemma conv_context_convp :
+  Lemma conv_cum_context_convp :
     forall Γ Γ' leq u v,
-      conv leq Σ Γ u v ->
+      conv_cum leq Σ Γ u v ->
       conv_context Σ Γ Γ' ->
-      conv leq Σ Γ' u v.
+      conv_cum leq Σ Γ' u v.
   Proof.
     intros Γ Γ' leq u v h hx.
     destruct hΣ.
     destruct leq.
     - simpl. destruct h. constructor.
-      eapply conv_alt_conv_ctx. all: eauto.
+      eapply conv_conv_ctx. all: eauto.
     - simpl in *. destruct h. constructor.
       eapply cumul_conv_ctx. all: eauto.
   Qed.
